template-coq/theories/Substitution.v
@@ -604,7 +604,9 @@ Require Import Weakening.
 Lemma subst_instantiate_params_subst n k params args s t :
   Forall Ast.wf n -> forall s' t',
     instantiate_params_subst params args s t = Some (s', t') ->
-    instantiate_params_subst params (map (subst n k) args) (map (subst n k) s) (subst n (#|s| + k) t) =
+    instantiate_params_subst
+      (mapi_rec (fun k' decl => subst_decl n (k' + k) decl) params #|s|)
+      (map (subst n k) args) (map (subst n k) s) (subst n (#|s| + k) t) =
     Some (map (subst n k) s', subst n (#|s| + k + #|params|) t').
 Proof.
   intros Hn.
@@ -627,22 +629,44 @@ Proof.
        rewrite <- IHparams. f_equal.
 Qed.
 
-Lemma subst_instantiate_params n k params args t :
-  Forall Ast.wf n -> forall t',
-    instantiate_params params args t = Some t' ->
-    instantiate_params params (map (subst n k) args) (subst n k t) =
-    Some (subst n k t').
+Require Import ssreflect ssrbool.
+
+Lemma subst_decl_closed n k d : wf_decl d -> closed_decl k d -> subst_decl n k d = d.
 Proof.
-  intros Hn t'. unfold instantiate_params.
-  generalize (subst_instantiate_params_subst n k params args [] t Hn).
-  destruct instantiate_params_subst as [[s' t'']|].
-  - intros Heq. specialize (Heq _ _ eq_refl). simpl in Heq. rewrite Heq.
-    intros [= <-].
-    rewrite distr_subst; auto. eapply instantiate_params_subst_length in Heq.
-    simpl in Heq; rewrite map_length in Heq. rewrite Heq. do 3 f_equal. lia.
-  - congruence.
+  case: d => na [body|] ty; rewrite /closed_decl /subst_decl /map_decl /wf_decl /= => [[wfb wfty]].
+  move/andP => [cb cty]. rewrite !subst_closedn //.
+  move=> cty; now rewrite !subst_closedn //.
 Qed.
-Hint Rewrite subst_instantiate_params : subst.
+
+Lemma closed_decl_upwards k d : closed_decl k d -> forall k', k <= k' -> closed_decl k' d.
+Proof.
+  case: d => na [body|] ty; rewrite /closed_decl /=.
+  move/andP => [cb cty] k' lek'. do 2 rewrite (closed_upwards k) //.
+  move=> cty k' lek'; rewrite (closed_upwards k) //.
+Qed.
+
+Lemma closed_ctx_subst n k ctx : Forall wf_decl ctx -> closed_ctx ctx = true -> subst_context n k ctx = ctx.
+Proof.
+  induction ctx in n, k |- *; auto.
+  unfold closed_ctx, id. intros wfctx. inv wfctx.
+  rewrite mapi_app forallb_app List.rev_length /= Nat.add_0_r.
+  move/andb_true_iff => /= [Hctx /andb_true_iff [Ha _]].
+  rewrite subst_context_snoc /snoc /= IHctx // subst_decl_closed //.
+  now apply: closed_decl_upwards.
+Qed.
+
+Lemma closed_tele_subst n k ctx :
+  Forall wf_decl ctx -> closed_ctx ctx ->
+  mapi (fun (k' : nat) (decl : context_decl) => subst_decl n (k' + k) decl) (List.rev ctx) = List.rev ctx.
+Proof.
+  rewrite /closed_ctx /mapi. generalize 0.
+  induction ctx using rev_ind; try easy.
+  move=> n0 /Forall_app [wfctx wfx]. inv wfx.
+  rewrite /closed_ctx !rev_app_distr /id /=.
+  move/andP => [closedx Hctx].
+  rewrite subst_decl_closed //. rewrite (closed_decl_upwards n0) //; lia.
+  f_equal. now rewrite IHctx.
+Qed.
 
 Lemma decompose_prod_n_assum_subst_ind ctx0 ctx1 ctx2 ctx3 n t s t' :
   Forall Ast.wf s ->
@@ -687,6 +711,17 @@ Proof.
   rewrite <- app_assoc. reflexivity.
 Qed.
 
+Lemma decompose_prod_n_assum_extend_ctx {ctx n t ctx' t'} ctx'' :
+  decompose_prod_n_assum ctx n t = Some (ctx', t') ->
+  decompose_prod_n_assum (ctx ++ ctx'') n t = Some (ctx' ++ ctx'', t').
+Proof.
+  induction n in ctx, t, ctx', t', ctx'' |- *. simpl. intros [= -> ->]. eauto.
+  simpl.
+  destruct (strip_outer_cast t); simpl; try congruence.
+  intros H. eapply (IHn _ _ _ _ ctx'' H).
+  intros H. eapply (IHn _ _ _ _ ctx'' H).
+Qed.
+
 Lemma decompose_prod_n_assum_subst ctx0 ctx1 ctx3 n t s t' :
   Forall Ast.wf s ->
   decompose_prod_n_assum (ctx0 ,,, ctx1) n t = Some (ctx0 ,,, ctx1 ,,, ctx3, t') ->
@@ -698,54 +733,6 @@ Proof.
   simpl in *. specialize (H1 H0). auto.
 Qed.
 
-(* Lemma subst_instantiate_params_none n k params args t : *)
-(*   Forall Ast.wf n -> has_nparams #|params| t -> Forall Ast.wf args -> Ast.wf t -> *)
-(*   instantiate_params params args t = None -> *)
-(*   instantiate_params params (map (subst n k) args) (subst n k t) = None. *)
-(* Proof. *)
-(*   intros Hn Hp Hargs Ht. *)
-(*   apply has_nparams_ex in Hp as [[ctx' t'] He]. *)
-(*   revert ctx' t' He. generalize (@nil context_decl). *)
-(*   induction params in args, Hargs, Hn, t, Ht, n, k |- *. *)
-(*   destruct args; simpl. discriminate. reflexivity. *)
-
-(*   simpl. *)
-(*   pose proof (strip_outer_cast_tProd_tLetIn_subst n t k) as Hsubst. *)
-(*   intros l' ctx' t'. *)
-(*   destruct (strip_outer_cast t) eqn:Hstript; try congruence; try reflexivity; try rewrite Hsubst. *)
-(*   destruct args; simpl; try congruence; auto. *)
-(*   - intros Ht'. *)
-(*     pose proof (decompose_prod_n_assum_ctx _ _ _ _ _ Ht') as [ctx'' ->]. *)
-(*     change (l',, vass n0 t0_1 ,,, ctx'') with (l' ,,, [vass n0 t0_1] ,,, ctx'') in Ht'. *)
-(*     change (l' ,, vass n0 t0_1) with (l' ,,, [vass n0 t0_1]) in Ht'. *)
-(*     eapply (decompose_prod_n_assum_subst _ _ _ _ _ [t0]) in Ht'. *)
-(*     inv Hargs. *)
-(*     assert (Ast.wf ((subst0 [t0]) t0_2)). apply wf_subst. wf. *)
-(*     apply wf_strip_outer_cast in Ht. rewrite Hstript in Ht. *)
-(*     now inv Ht. *)
-(*     specialize (IHparams n k args _ Hn H0 H1 _ _ _ Ht'). *)
-(*     unfold subst1 in *. *)
-(*     intros. destruct (decl_body a); try congruence. specialize (IHparams H2). *)
-(*     rewrite <- IHparams. f_equal. *)
-(*     now rewrite distr_subst. *)
-(*     now inv Hargs. *)
-(*   - intros Ht'. *)
-(*     pose proof (decompose_prod_n_assum_ctx _ _ _ _ _ Ht') as [ctx'' ->]. *)
-(*     change (l',, vdef n0 t0_1 t0_2 ,,, ctx'') with (l' ,,, [vdef n0 t0_1 t0_2] ,,, ctx'') in Ht'. *)
-(*     change (l' ,, vdef n0 t0_1 t0_2) with (l' ,,, [vdef n0 t0_1 t0_2]) in Ht'. *)
-(*     eapply (decompose_prod_n_assum_subst _ _ _ _ _ [t0_1]) in Ht'. *)
-(*     assert (Ast.wf ((subst0 [t0_1]) t0_3)). *)
-(*     apply wf_strip_outer_cast in Ht. rewrite Hstript in Ht. *)
-(*     inv Ht; now apply wf_subst. *)
-(*     specialize (IHparams n k args _ Hn Hargs H _ _ _ Ht'). *)
-(*     unfold subst1 in *. *)
-(*     intros. destruct (decl_body a); try congruence. specialize (IHparams H0). *)
-(*     rewrite <- IHparams. f_equal. *)
-(*     now rewrite distr_subst. *)
-(*     apply wf_strip_outer_cast in Ht. rewrite Hstript in Ht. *)
-(*     now inv Ht. *)
-(* Qed. *)
-
 Lemma subst_it_mkProd_or_LetIn n k ctx t :
   subst n k (it_mkProd_or_LetIn ctx t) =
   it_mkProd_or_LetIn (subst_context n k ctx) (subst n (length ctx + k) t).
@@ -756,24 +743,27 @@ Proof.
   pose (subst_context_snoc n k ctx a). simpl. now rewrite IHctx.
 Qed.
 
-Lemma to_extended_list_subst n k c :
-  to_extended_list (subst_context n k c) = to_extended_list c.
+Lemma to_extended_list_k_subst n k c k' :
+  to_extended_list_k (subst_context n k c) k' = to_extended_list_k c k'.
 Proof.
-  unfold to_extended_list. generalize 0. generalize (@nil term) at 1 2.
+  unfold to_extended_list_k. revert k'.
+  generalize (@nil term) at 1 2.
   induction c in n, k |- *; simpl; intros. reflexivity.
   rewrite subst_context_snoc. unfold snoc. simpl.
   destruct a. destruct decl_body. unfold subst_decl, map_decl. simpl.
   now rewrite IHc. simpl. apply IHc.
 Qed.
 
-Lemma to_extended_list_map_subst:
-  forall n (k : nat) (c : context), to_extended_list c = map (subst n (#|c| + k)) (to_extended_list c).
+Lemma to_extended_list_k_map_subst:
+  forall n (k : nat) (c : context) k',
+    #|c| + k' <= k ->
+    to_extended_list_k c k' = map (subst n k) (to_extended_list_k c k').
 Proof.
-  intros n k c.
-  pose proof (to_extended_list_lift_above c).
+  intros n k c k'.
+  pose proof (to_extended_list_k_spec c k').
   symmetry. apply_spec. intros.
-  destruct H0. intuition. subst x. simpl.
-  destruct (leb_spec_Set (#|c| + k) x0). lia. reflexivity.
+  destruct H1. intuition. subst x. simpl.
+  destruct (leb_spec_Set k x0). lia. reflexivity.
 Qed.
 
 Lemma Alli_mapi_spec {A B} {P : nat -> A -> Type} {l} {f g : nat -> A -> B} {n} :
@@ -784,18 +774,106 @@ Proof.
   intros Heq. rewrite Heq; f_equal; auto.
 Qed.
 
+Lemma subst_instantiate_params_none n k params args s t :
+  Forall Ast.wf n -> has_nparams #|params| t -> Forall Ast.wf args -> Ast.wf t ->
+  instantiate_params_subst params args s t = None ->
+  instantiate_params_subst params (map (subst n k) args) s (subst n k t) = None.
+Proof.
+  intros Hn Hp Hargs Ht.
+  apply has_nparams_ex in Hp as [[ctx' t'] He].
+  revert ctx' t' He. generalize (@nil context_decl).
+  induction params in args, Hargs, Hn, t, Ht, n, k |- *.
+  destruct args; simpl. discriminate. reflexivity.
+
+  (* simpl. *)
+  (* pose proof (strip_outer_cast_tProd_tLetIn_subst n t k) as Hsubst. *)
+  (* intros l' ctx' t'. *)
+  (* destruct (strip_outer_cast t) eqn:Hstript; try congruence; try reflexivity; try rewrite Hsubst. *)
+  (* destruct args; simpl; try congruence; auto. *)
+  (* unfold instantiate_params. simpl. *)
+  (* - intros Ht'. *)
+  (*   pose proof (decompose_prod_n_assum_ctx _ _ _ _ _ Ht') as [ctx'' ->]. *)
+  (*   change (l',, vass n0 t0_1 ,,, ctx'') with (l' ,,, [vass n0 t0_1] ,,, ctx'') in Ht'. *)
+  (*   change (l' ,, vass n0 t0_1) with (l' ,,, [vass n0 t0_1]) in Ht'. *)
+  (*   eapply (decompose_prod_n_assum_subst _ _ _ _ _ [t0_1]) in Ht'. *)
+  (*   inv Hargs. *)
+  (*   assert (Ast.wf ((subst0 [t0_1]) t0_2)). apply wf_subst. admit. admit. *)
+  (*   apply wf_strip_outer_cast in Ht. rewrite Hstript in Ht. *)
+  (*   (* now inv Ht. *) *)
+  (*   specialize (IHparams n k args _ Hn H0 H _ _ _ Ht'). *)
+  (*   unfold subst1 in *. *)
+  (*   intros. destruct (decl_body a); try congruence. specialize (IHparams H2). *)
+  (*   rewrite <- IHparams. f_equal. *)
+  (*   now rewrite distr_subst. *)
+  (*   now inv Hargs. *)
+  (* - intros Ht'. *)
+  (*   pose proof (decompose_prod_n_assum_ctx _ _ _ _ _ Ht') as [ctx'' ->]. *)
+  (*   change (l',, vdef n0 t0_1 t0_2 ,,, ctx'') with (l' ,,, [vdef n0 t0_1 t0_2] ,,, ctx'') in Ht'. *)
+  (*   change (l' ,, vdef n0 t0_1 t0_2) with (l' ,,, [vdef n0 t0_1 t0_2]) in Ht'. *)
+  (*   eapply (decompose_prod_n_assum_subst _ _ _ _ _ [t0_1]) in Ht'. *)
+  (*   assert (Ast.wf ((subst0 [t0_1]) t0_3)). *)
+  (*   apply wf_strip_outer_cast in Ht. rewrite Hstript in Ht. *)
+  (*   inv Ht; now apply wf_subst. *)
+  (*   specialize (IHparams n k args _ Hn Hargs H _ _ _ Ht'). *)
+  (*   unfold subst1 in *. *)
+  (*   intros. destruct (decl_body a); try congruence. specialize (IHparams H0). *)
+  (*   rewrite <- IHparams. f_equal. *)
+  (*   now rewrite distr_subst. *)
+  (*   apply wf_strip_outer_cast in Ht. rewrite Hstript in Ht. *)
+  (*   now inv Ht. *)
+Admitted.
+
+Lemma subst_instantiate_params n k params args t :
+  Forall wf_decl params -> Forall Ast.wf n -> Forall Ast.wf args -> Ast.wf t ->
+  closed_ctx params ->
+  option_map (subst n k) (instantiate_params params args t) =
+  instantiate_params params (map (subst n k) args) (subst n k t).
+Proof.
+  unfold instantiate_params.
+  move=> wfparams wfn wfargs wft.
+  move/(closed_tele_subst n k params)=> Heq.
+  rewrite -{2}Heq //.
+  specialize (subst_instantiate_params_subst n k (List.rev params) args [] t wfn).
+  move=> /= Heq'.
+  case E: (instantiate_params_subst (List.rev params) args)=> [[l' t']|] /= //.
+  specialize (Heq' _ _ E). rewrite Heq'. f_equal.
+  rewrite distr_subst //.
+  move/instantiate_params_subst_length: E => -> /=. do 2 f_equal. lia.
+  rewrite Heq; auto.
+  eapply subst_instantiate_params_none in E. rewrite -> E. reflexivity. eauto. admit. auto. auto.
+Admitted.
+Hint Rewrite subst_instantiate_params : lift.
+
+(* Lemma subst_instantiate_params n k params args t : *)
+(*   Forall Ast.wf n -> closed_ctx params = true -> *)
+(*   forall t', *)
+(*     instantiate_params params args t = Some t' -> *)
+(*     instantiate_params params (map (subst n k) args) (subst n k t) = *)
+(*     Some (subst n k t'). *)
+(* Proof. *)
+(*   intros Hn Hpars t'. unfold instantiate_params. *)
+(*   generalize (subst_instantiate_params_subst n k params args [] t Hn). *)
+(*   destruct instantiate_params_subst as [[s' t'']|]. *)
+(*   - intros Heq. specialize (Heq _ _ eq_refl). simpl in Heq. rewrite Heq. *)
+(*     intros [= <-]. *)
+(*     rewrite distr_subst; auto. eapply instantiate_params_subst_length in Heq. *)
+(*     simpl in Heq; rewrite map_length in Heq. rewrite Heq. do 3 f_equal. lia. *)
+(*   - congruence. *)
+(* Qed. *)
+(* Hint Rewrite subst_instantiate_params : subst. *)
+
 Lemma has_nparams_subst n t s k : has_nparams n t -> has_nparams n (subst s k t).
 Proof.
   intros H. eapply subst_decompose_prod_n_assum in H.
   destruct decompose_prod_n_assum. destruct p as [ctx' t'].
-  red. rewrite H. congruence. elim H.
+  red. rewrite -> H. congruence. elim H.
 Qed.
 
 Lemma has_nparams_subst_instance_constr n t u : has_nparams n t -> has_nparams n (subst_instance_constr u t).
 Proof.
   intros H. eapply subst_instance_constr_decompose_prod_n_assum in H.
   destruct decompose_prod_n_assum. destruct p as [ctx' t'].
-  red. rewrite H. congruence. elim H.
+  red. rewrite -> H. congruence. elim H.
 Qed.
 
 Lemma subst_instance_constr_it_mkProd_or_LetIn u ctx t :
@@ -876,9 +954,9 @@ Proof.
   now rewrite app_context_nil_l.
   simpl in X.
   eapply (env_prop_typing _ typecheck_closed) in Hs; eauto.
-  rewrite andb_true_iff in Hs. destruct Hs as [Hs Ht].
+  rewrite -> andb_true_iff in Hs. destruct Hs as [Hs Ht].
   simpl in Hs. apply (lift_closed #|arities_context l|) in Hs.
-  rewrite Hs, app_context_nil_l in X.
+  rewrite -> Hs, app_context_nil_l in X.
   apply X.
 Qed.
 
@@ -893,29 +971,29 @@ Proof.
   destruct cdecl as [[id cty] car].
   eapply (env_prop_typing _ typecheck_closed) in Hs; eauto.
   rewrite arities_context_length in Hs.
-  rewrite andb_true_iff in *. simpl in *.
+  rewrite -> andb_true_iff in *. simpl in *.
   destruct Hs as [Hs _].
   unfold substl. eapply (closedn_subst _ 0 0).
   clear. unfold inds. induction #|ind_bodies mdecl|; simpl; try constructor; auto.
-  simpl. now rewrite inds_length, closedn_subst_instance_constr.
+  simpl. now rewrite -> inds_length, closedn_subst_instance_constr.
 Qed.
 
 Lemma simpl_subst_k (N : list term) (M : term) :
   Ast.wf M -> forall k p, p = #|N| -> subst N k (lift p k M) = M.
 Proof.
   intros. subst p. rewrite <- (Nat.add_0_r #|N|).
-  rewrite simpl_subst_rec, lift0_id; auto. Qed.
+  rewrite -> simpl_subst_rec, lift0_id; auto. Qed.
 
 Ltac nth_leb_simpl :=
   match goal with
     |- context [leb ?k ?n] => elim (leb_spec_Set k n); try lia; intros; simpl
-  | |- context [nth_error ?l ?n] => elim (nth_error_spec l n); rewrite ?app_length, ?map_length;
+  | |- context [nth_error ?l ?n] => elim (nth_error_spec l n); rewrite -> ?app_length, ?map_length;
                                     try lia; intros; simpl
   | H : context[nth_error (?l ++ ?l') ?n] |- _ =>
-    (rewrite (AstUtils.nth_error_app_ge l l' n) in H by lia) ||
-    (rewrite (AstUtils.nth_error_app_lt l l' n) in H by lia)
+    (rewrite -> (AstUtils.nth_error_app_ge l l' n) in H by lia) ||
+    (rewrite -> (AstUtils.nth_error_app_lt l l' n) in H by lia)
   | H : nth_error ?l ?n = Some _, H' : nth_error ?l ?n' = Some _ |- _ =>
-    replace n' with n in H' by lia; rewrite H in H'; injection H'; intros; subst
+    replace n' with n in H' by lia; rewrite -> H in H'; injection H'; intros; subst
   | _ => lia || congruence || solve [repeat (f_equal; try lia)]
   end.
 
@@ -931,15 +1009,15 @@ Proof.
   intros wft wfl.
   induction wft in k |- * using term_wf_forall_list_ind; simpl; auto;
     rewrite ?subst_mkApps; try change_Sk;
-    try (f_equal; rewrite ?map_map_compose, ?compose_on_snd, ?compose_map_def, ?map_length;
+    try (f_equal; rewrite -> ?map_map_compose, ?compose_on_snd, ?compose_map_def, ?map_length;
          eauto; apply_spec; eauto).
 
   - repeat nth_leb_simpl.
     rewrite nth_error_map in e0. rewrite e in e0.
     injection e0; intros <-.
-    rewrite permute_lift, Nat.add_0_r by auto.
+    rewrite -> permute_lift, Nat.add_0_r by auto.
     rewrite <- (Nat.add_0_r #|l'|).
-    rewrite simpl_subst_rec, lift0_id; auto with wf; try lia. apply wf_lift.
+    rewrite -> simpl_subst_rec, lift0_id; auto with wf; try lia. apply wf_lift.
     eapply nth_error_forall in e; eauto.
 Qed.
 
@@ -950,11 +1028,11 @@ Proof.
   intros wft wfl wfl'.
   induction wft in k |- * using term_wf_forall_list_ind; simpl; eauto;
     rewrite ?subst_mkApps; try change_Sk;
-    try (f_equal; rewrite ?map_map_compose, ?compose_on_snd, ?compose_map_def, ?map_length, ?Nat.add_assoc;
+    try (f_equal; rewrite -> ?map_map_compose, ?compose_on_snd, ?compose_map_def, ?map_length, ?Nat.add_assoc;
          eauto; apply_spec; eauto).
 
   - repeat nth_leb_simpl.
-    rewrite Nat.add_comm, simpl_subst; eauto.
+    rewrite -> Nat.add_comm, simpl_subst; eauto.
     eapply nth_error_forall in e; eauto.
 Qed.
 
@@ -978,6 +1056,9 @@ Inductive context_subst : context -> list term -> list term -> Set :=
 Lemma context_subst_length Γ a s : context_subst Γ a s -> #|Γ| = #|s|.
 Proof. induction 1; simpl; congruence. Qed.
 
+Lemma context_subst_assumptions_length Γ a s : context_subst Γ a s -> context_assumptions Γ = #|a|.
+Proof. induction 1; simpl; try congruence. rewrite app_length /=. lia. Qed.
+
 Lemma context_subst_app `{cf:checker_flags} Σ Γ Γ' a s :
   All_local_env (fun _ _ t T => Ast.wf t /\ Ast.wf T) Σ Γ' ->
   Forall Ast.wf a -> Forall Ast.wf s ->
@@ -1000,12 +1081,12 @@ Proof.
     specialize (IHΓ' _ _ _ H0 wfa Hs0 H).
     destruct IHΓ' as (a0' & a1' & s1 & s2 & ((sa0 & sa1) & eqargs) & eqs0).
     subst. exists a0', a1', s1, (subst s2 0 (subst s1 #|Γ'| b) :: s2). intuition eauto.
-    rewrite subst_context_snoc, Nat.add_0_r.
+    rewrite -> subst_context_snoc, Nat.add_0_r.
     unfold subst_decl; simpl. unfold map_decl. simpl.
     econstructor. auto. simpl. f_equal.
-    rewrite subst_app_simpl; auto. simpl.
+    rewrite -> subst_app_simpl; auto. simpl.
     pose proof(context_subst_length _ _ _ sa1) as Hs1.
-    rewrite subst_context_length in Hs1. rewrite Hs1. auto. auto.
+    rewrite subst_context_length in Hs1. rewrite -> Hs1. auto. auto.
     apply Forall_app in Hs0. intuition.
     apply Forall_app in Hs0. intuition.
 Qed.
@@ -1014,90 +1095,372 @@ Lemma it_mkProd_or_LetIn_app l l' t :
   it_mkProd_or_LetIn (l ++ l') t = it_mkProd_or_LetIn l' (it_mkProd_or_LetIn l t).
 Proof. induction l in l', t |- *; simpl; auto. Qed.
 
-Lemma instantiate_params_context_subst `{cf:checker_flags} Σ args parctx ty s :
-  All_local_env (fun _ _ t T => Ast.wf t /\ Ast.wf T) Σ parctx -> Ast.wf ty ->
-  Forall Ast.wf args -> Forall Ast.wf s -> forall s' t',
-  instantiate_params_subst (List.rev parctx) args s (it_mkProd_or_LetIn parctx ty) = Some (s', t') ->
-  (context_subst parctx args s' * (ty = t'))%type.
-Proof.
-  revert s args parctx ty.
-  refine (well_founded_ind (measure_wf lt_wf (@length term)) _ _).
-  intros s IH args parctx. destruct parctx using rev_ind; intros ty wfctx wfty wfargs wfs.
+(* Lemma instantiate_params_subst_pres {params args s t s' t'} : *)
+(*     instantiate_params_subst params args s t = Some (s', t') -> *)
+(*     {s'' & s' = s'' ++ s }. *)
+(* Proof. *)
+(*   induction params in args, s, t, s', t' |- *; simpl; intros. *)
+(*   destruct args; try congruence. exists []. simpl; congruence. *)
+(*   destruct (decl_body a); destruct (strip_outer_cast t); try congruence. *)
+(*   destruct (IHparams _ _ _ _ _ H) as [s'' ->]. *)
+(*   exists (s'' ++ [subst0 s t1_1]). now rewrite <- app_assoc. *)
+(*   destruct args; try congruence. *)
+(*   destruct (IHparams _ _ _ _ _ H) as [s'' ->]. *)
+(*   exists (s'' ++ [t0]). now rewrite <- app_assoc. *)
+(* Qed. *)
 
-Lemma instantiate_params_context_subst `{cf:checker_flags} Σ args parctx ty s :
-  All_local_env (fun _ _ t T => Ast.wf t /\ Ast.wf T) Σ parctx -> Ast.wf ty ->
-  Forall Ast.wf args -> Forall Ast.wf s ->
-  context_subst parctx args s ->
-  forall parctx' s', parctx = subst_context s' 0 parctx' ->
-  instantiate_params (List.rev parctx') args (it_mkProd_or_LetIn parctx ty) = Some (subst s 0 ty).
-Proof.
-  revert s args parctx ty.
-  refine (well_founded_ind (measure_wf lt_wf (@length term)) _ _).
-  intros s IH args parctx. destruct parctx using rev_ind; intros ty wfctx wfty wfargs wfs.
+(* Lemma instantiate_params_context_subst `{cf:checker_flags} Σ args ctx ty s : *)
+(*   Ast.wf ty -> *)
+(*   Forall Ast.wf args -> Forall Ast.wf s -> *)
+(*   context_subst ctx args s -> forall ctx' args' s' t' *)
+(*   (wfctx' : All_local_env (fun _ _ t T => Ast.wf t /\ Ast.wf T) Σ ctx'), *)
+(*   instantiate_params_subst (List.rev ctx') args' s ty = Some (s', t') -> *)
+(*   (context_subst (ctx' ++ ctx) (args ++ args') s' * (ty = t'))%type. *)
+(* Proof. *)
+(*   intros wfty wfargs wfs Hs ctx'. *)
+(*   revert ctx args wfargs ty wfty s wfs Hs. *)
+(*   induction ctx' using rev_ind; intros. (* in ctx, args, s, ty, Hs |- *; intros. *) *)
+(*   - simpl in H. destruct args'; try congruence. simpl. *)
+(*     revert H. intros [= -> ->]. rewrite app_nil_r; intuition. *)
+(*   - simpl in H. *)
+(*     rewrite rev_app_distr in H. simpl in H. *)
+(*     destruct x as [na [body|] ty']. simpl in *. *)
+(*     destruct (strip_outer_cast ty) eqn:Heq; try discriminate. *)
+(*     split. *)
+(*     specialize (IHctx' (vdef na body ty' :: ctx) args wfargs ty'). *)
+(*     forward IHctx'. admit. *)
+(*     destruct (instantiate_params_subst_pres H) as [s'' ->]. *)
+(*     specialize (IHctx' (subst0 s t1 :: s)). *)
+(*     forward IHctx'. constructor; auto. apply wf_subst; auto. admit. *)
+(*     forward IHctx'. constructor; auto. *)
+(*     specialize (IHctx' args' _ _ H). *)
+(*     rewrite <- app_assoc. simpl. *)
 
-Lemma context_subst_instantiate_params `{cf:checker_flags} Σ args parctx ty s :
-  All_local_env (fun _ _ t T => Ast.wf t /\ Ast.wf T) Σ parctx -> Ast.wf ty ->
-  Forall Ast.wf args -> Forall Ast.wf s ->
-  context_subst parctx args s ->
-  forall parctx' s', parctx = subst_context s' 0 parctx' ->
-  instantiate_params (List.rev parctx') args (it_mkProd_or_LetIn parctx ty) = Some (subst s 0 ty).
-Proof.
-  revert s args parctx ty.
-  refine (well_founded_ind (measure_wf lt_wf (@length term)) _ _).
-  intros s IH args parctx. destruct parctx using rev_ind; intros ty wfctx wfty wfargs wfs.
-  - intros H; inv H. simpl; rewrite subst_empty; auto.
-    intros. destruct parctx'; simpl in *; try congruence. rewrite subst_context_snoc in H. discriminate.
-  - intros Hcsubst. clear IHparctx.
-    apply All_local_env_app in wfctx as [wfd wfctx].
-    eapply context_subst_app in Hcsubst; eauto.
-    destruct Hcsubst as (a0 & a1 & s0 & s1 & (((Hd & Hs1) & eqargs) & eqs)).
-    rewrite it_mkProd_or_LetIn_app. simpl.
-    intros parctx' s' Hparctx'.
-    destruct x as [na [body|] dty]; simpl in *.
-    destruct parctx' using rev_ind;
-    [apply app_eq_nil in Hparctx'; intuition discriminate|
-    clear IHparctx'; unfold subst_context in Hparctx'; simpl in Hparctx';
-    rewrite fold_context_app in Hparctx'; apply app_inj_tail in Hparctx' as [Hparctx' Hd']].
-    rewrite rev_app_distr.
-    inversion wfd.
-    -- subst Γ b t na0. simpl. simpl in Hd'. destruct x as [na' [body'|] ty']; try discriminate. simpl.
-       injection Hd'. intros -> -> <-.
-       unfold subst1. rewrite subst_it_mkProd_or_LetIn.
-       subst s args. revert IH Hs1. inv Hd. inv H. intros IH Hs1. simpl.
-       specialize (IH s1).
-       forward IH. red. rewrite app_length. simpl. lia.
-       rewrite subst_empty in *; intuition auto.
-       specialize (IH a1 (subst_context [subst0 s' body'] 0 l) (subst [subst0 s' body'] #|l| ty)).
-       eapply Forall_app in wfs as [wfs1 wfs0]. eapply Forall_app in wfargs as [wfa0 wfa1].
-       forward IH.
-       { rewrite subst_context_alt.
-         clear -wfctx wfs0 H.
-         generalize #|l|. unfold mapi. generalize 0 at 3.
-         induction wfctx; econstructor; intuition eauto with wf. }
-       do 3 forward IH; intuition auto with wf.
-       specialize (H2 l [subst0 s' body'] eq_refl).
-       rewrite Nat.add_0_r. rewrite H2.
-       f_equal.
-       rewrite subst_app_simpl; auto. simpl.
-       apply context_subst_length in Hs1. rewrite subst_context_length in Hs1. now rewrite Hs1.
+(* Lemma instantiate_params_context_subst `{cf:checker_flags} Σ args parctx ty s : *)
+(*   All_local_env (fun _ _ t T => Ast.wf t /\ Ast.wf T) Σ parctx -> Ast.wf ty -> *)
+(*   Forall Ast.wf args -> Forall Ast.wf s -> *)
+(*   context_subst parctx args s -> *)
+(*   forall parctx' s', parctx = subst_context s' 0 parctx' -> *)
+(*   instantiate_params (List.rev parctx') args (it_mkProd_or_LetIn parctx ty) = Some (subst s 0 ty). *)
+(* Proof. *)
+(*   revert s args parctx ty. *)
+(*   refine (well_founded_ind (measure_wf lt_wf (@length term)) _ _). *)
+(*   intros s IH args parctx. destruct parctx using rev_ind; intros ty wfctx wfty wfargs wfs. *)
 
-    -- subst args s. simpl. revert IH wfs Hs1. inv Hd. inv H. intros.
-       simpl.
-       unfold subst1. rewrite subst_it_mkProd_or_LetIn.
-       specialize (IH s1).
-       forward IH. red. rewrite app_length. simpl. lia.
-       specialize (IH a1 (subst_context [a] 0 l) (subst [a] #|l| ty)).
-       eapply Forall_app in wfs as [wfs1 wfs0]. inv wfs0. eapply Forall_app in wfargs as [wfa0 wfa1].
-       forward IH.
-       { rewrite subst_context_alt.
-         clear -wfctx H.
-         generalize #|l|. unfold mapi. generalize 0 at 2.
-         induction wfctx; econstructor; intuition eauto with wf. }
-       do 3 forward IH; intuition auto with wf.
-       rewrite subst_context_length in H1.
-       rewrite Nat.add_0_r, H1. f_equal.
-       rewrite subst_app_simpl; auto.
-       apply context_subst_length in Hs1. rewrite subst_context_length in Hs1. now rewrite Hs1.
+(* Lemma context_subst_instantiate_params `{cf:checker_flags} Σ args parctx ty s : *)
+(*   All_local_env (fun _ _ t T => Ast.wf t /\ Ast.wf T) Σ parctx -> Ast.wf ty -> *)
+(*   Forall Ast.wf args -> Forall Ast.wf s -> *)
+(*   context_subst parctx args s -> *)
+(*   forall parctx' s', parctx = subst_context s' 0 parctx' -> *)
+(*   instantiate_params (List.rev parctx') args (it_mkProd_or_LetIn parctx ty) = Some (subst s 0 ty). *)
+(* Proof. *)
+(*   revert s args parctx ty. *)
+(*   refine (well_founded_ind (measure_wf lt_wf (@length term)) _ _). *)
+(*   intros s IH args parctx. destruct parctx using rev_ind; intros ty wfctx wfty wfargs wfs. *)
+(*   - intros H; inv H. simpl; rewrite subst_empty; auto. *)
+(*     intros. destruct parctx'; simpl in *; try congruence. rewrite -> subst_context_snoc in H. discriminate. *)
+(*   - intros Hcsubst. clear IHparctx. *)
+(*     apply All_local_env_app in wfctx as [wfd wfctx]. *)
+(*     eapply context_subst_app in Hcsubst; eauto. *)
+(*     destruct Hcsubst as (a0 & a1 & s0 & s1 & (((Hd & Hs1) & eqargs) & eqs)). *)
+(*     rewrite it_mkProd_or_LetIn_app. simpl. *)
+(*     intros parctx' s' Hparctx'. *)
+(*     destruct x as [na [body|] dty]; simpl in *. *)
+(*     destruct parctx' using rev_ind; *)
+(*     [apply app_eq_nil in Hparctx'; intuition discriminate| *)
+(*     clear IHparctx'; unfold subst_context in Hparctx'; simpl in Hparctx'; *)
+(*     rewrite fold_context_app in Hparctx'; apply app_inj_tail in Hparctx' as [Hparctx' Hd']]. *)
+(*     rewrite rev_app_distr. *)
+(*     inversion wfd. *)
+(*     -- subst Γ b t na0. simpl. simpl in Hd'. destruct x as [na' [body'|] ty']; try discriminate. simpl. *)
+(*        injection Hd'. intros -> -> <-. *)
+(*        unfold subst1. rewrite subst_it_mkProd_or_LetIn. *)
+(*        subst s args. revert IH Hs1. inv Hd. inv H. intros IH Hs1. simpl. *)
+(*        specialize (IH s1). *)
+(*        forward IH. red. rewrite app_length. simpl. lia. *)
+(*        rewrite subst_empty in *; intuition auto. *)
+(*        specialize (IH a1 (subst_context [subst0 s' body'] 0 l) (subst [subst0 s' body'] #|l| ty)). *)
+(*        eapply Forall_app in wfs as [wfs1 wfs0]. eapply Forall_app in wfargs as [wfa0 wfa1]. *)
+(*        forward IH. *)
+(*        { rewrite subst_context_alt. *)
+(*          clear -wfctx wfs0 H. *)
+(*          generalize #|l|. unfold mapi. generalize 0 at 3. *)
+(*          induction wfctx; econstructor; intuition eauto with wf. } *)
+(*        do 3 forward IH; intuition auto with wf. *)
+(*        specialize (H2 l [subst0 s' body'] eq_refl). *)
+(*        rewrite Nat.add_0_r. rewrite H2. *)
+(*        f_equal. *)
+(*        rewrite subst_app_simpl; auto. simpl. *)
+(*        apply context_subst_length in Hs1. rewrite subst_context_length in Hs1. now rewrite Hs1. *)
+
+(*     -- subst args s. simpl. revert IH wfs Hs1. inv Hd. inv H. intros. *)
+(*        simpl. *)
+(*        unfold subst1. rewrite subst_it_mkProd_or_LetIn. *)
+(*        specialize (IH s1). *)
+(*        forward IH. red. rewrite app_length. simpl. lia. *)
+(*        specialize (IH a1 (subst_context [a] 0 l) (subst [a] #|l| ty)). *)
+(*        eapply Forall_app in wfs as [wfs1 wfs0]. inv wfs0. eapply Forall_app in wfargs as [wfa0 wfa1]. *)
+(*        forward IH. *)
+(*        { rewrite subst_context_alt. *)
+(*          clear -wfctx H. *)
+(*          generalize #|l|. unfold mapi. generalize 0 at 2. *)
+(*          induction wfctx; econstructor; intuition eauto with wf. } *)
+(*        do 3 forward IH; intuition auto with wf. *)
+(*        rewrite subst_context_length in H1. *)
+(*        rewrite Nat.add_0_r, H1. f_equal. *)
+(*        rewrite subst_app_simpl; auto. *)
+(*        apply context_subst_length in Hs1. rewrite subst_context_length in Hs1. now rewrite Hs1. *)
+(* Qed. *)
+
+Fixpoint make_context_subst ctx args s :=
+  match ctx with
+  | [] => match args with
+          | [] => Some s
+          | a :: args => None
+          end
+  | d :: ctx =>
+    match d.(decl_body) with
+    | Some body => make_context_subst ctx args (subst0 s body :: s)
+    | None => match args with
+              | a :: args => make_context_subst ctx args (a :: s)
+              | [] => None
+              end
+    end
+  end.
+
+Lemma make_context_subst_rec_spec ctx args s tele args' s' :
+  context_subst ctx args s ->
+  make_context_subst tele args' s = Some s' ->
+  context_subst (List.rev tele ++ ctx) (args ++ args') s'.
+Proof.
+  induction tele in ctx, args, s, args', s' |- *.
+  - move=> /= Hc. case: args'. move => [= <-].
+    now rewrite app_nil_r.
+    move=> a l //.
+  - move=> Hc /=. case: a => [na [body|] ty] /=.
+    -- specialize (IHtele (vdef na body ty :: ctx) args (subst0 s body :: s) args' s').
+       move=> /=. rewrite <- app_assoc.
+       move/(IHtele _). move=> H /=. apply H.
+       constructor. auto.
+    -- case: args' => [|a args']; try congruence.
+       specialize (IHtele (vass na ty :: ctx) (args ++ [a]) (a :: s) args' s').
+       move=> /=. rewrite <- app_assoc.
+       move/(IHtele _). move=> H /=. simpl in H. rewrite <- app_assoc in H. apply H.
+       constructor. auto.
+Qed.
+
+Lemma make_context_subst_spec tele args s' :
+  make_context_subst tele args [] = Some s' ->
+  context_subst (List.rev tele) args s'.
+Proof.
+  move/(make_context_subst_rec_spec [] [] [] _ _ _ context_subst_nil).
+  rewrite app_nil_r /= //.
+Qed.
+
+Lemma instantiate_params_subst_make_context_subst ctx args s ty s' ty' :
+  instantiate_params_subst ctx args s ty = Some (s', ty') ->
+  exists ctx'',
+  make_context_subst ctx args s = Some s' /\
+  decompose_prod_n_assum [] (length ctx) ty = Some (ctx'', ty').
+Proof.
+  induction ctx in args, s, ty, s' |- *; simpl.
+  case: args => [|a args'] // [= <- <-]. exists []; intuition congruence.
+  case: a => [na [body|] ty''] /=.
+  - destruct (strip_outer_cast ty); try congruence.
+    intros. move: (IHctx _ _ _ _ H) => [ctx'' [Hmake Hdecomp]].
+    eapply (decompose_prod_n_assum_extend_ctx [vdef n t1 t2]) in Hdecomp.
+    unfold snoc. eexists; intuition eauto.
+  - destruct (strip_outer_cast ty); try congruence.
+    case: args => [|a args']; try congruence.
+    move=> H. move: (IHctx _ _ _ _ H) => [ctx'' [Hmake Hdecomp]].
+    eapply (decompose_prod_n_assum_extend_ctx [vass n t1]) in Hdecomp.
+    unfold snoc. eexists; intuition eauto.
+Qed.
+
+Lemma instantiate_params_make_context_subst ctx args ty ty' :
+  instantiate_params ctx args ty = Some ty' ->
+  exists ctx' ty'' s',
+    decompose_prod_n_assum [] (length ctx) ty = Some (ctx', ty'') /\
+    make_context_subst (List.rev ctx) args [] = Some s' /\ ty' = subst0 s' ty''.
+Proof.
+  unfold instantiate_params.
+  case E: instantiate_params_subst => [[s ty'']].
+  move=> [= <-].
+  eapply instantiate_params_subst_make_context_subst in E.
+  destruct E as [ctx'' [Hs Hty'']].
+  exists ctx'', ty'', s. split; auto.
+  now rewrite -> List.rev_length in Hty''.
+  congruence.
+Qed.
+
+Lemma decompose_prod_n_assum_it_mkProd ctx ctx' ty :
+  decompose_prod_n_assum ctx #|ctx'| (it_mkProd_or_LetIn ctx' ty) = Some (ctx' ++ ctx, ty).
+Proof.
+  revert ctx ty. induction ctx' using rev_ind; move=> // ctx ty.
+  rewrite app_length /= it_mkProd_or_LetIn_app /=.
+  destruct x as [na [body|] ty'] => /=;
+  now rewrite !Nat.add_1_r /= IHctx' -app_assoc.
+Qed.
+
+Definition is_ind_app_head t :=
+  match t with
+  | tInd _ _ => true
+  | tApp (tInd _ _) _ => true
+  | _ => false
+  end.
+
+Lemma is_ind_app_head_mkApps ind u l : is_ind_app_head (mkApps (tInd ind u) l).
+Proof. now destruct l; simpl. Qed.
+
+Lemma decompose_prod_assum_it_mkProd ctx ctx' ty :
+  is_ind_app_head ty ->
+  decompose_prod_assum ctx (it_mkProd_or_LetIn ctx' ty) = (ctx' ++ ctx, ty).
+Proof.
+  revert ctx ty. induction ctx' using rev_ind; move=> // ctx ty /=.
+  destruct ty; simpl; try (congruence || reflexivity).
+  move=> Hty. rewrite it_mkProd_or_LetIn_app /=.
+  case: x => [na [body|] ty'] /=; by rewrite IHctx' // /snoc -app_assoc.
+Qed.
+
+Lemma inds_alt ind u l :
+  inds ind u l = List.rev (mapi (fun i _ => tInd {| inductive_mind := ind; inductive_ind := i |} u) l).
+Proof.
+  unfold inds, mapi. induction l using rev_ind. simpl. reflexivity.
+  now rewrite app_length /= Nat.add_1_r IHl mapi_rec_app /= rev_app_distr /= Nat.add_0_r.
+Qed.
+
+Lemma map_subst_instance_constr_to_extended_list_k u ctx k :
+  map (subst_instance_constr u) (to_extended_list_k ctx k) = to_extended_list_k ctx k.
+Proof.
+  pose proof (to_extended_list_k_spec ctx k).
+  apply_spec. intros. now destruct H0 as [n [-> _]].
+Qed.
+
+Lemma subst_cstr_concl_head ind u mdecl (arity : context) args :
+  let head := tRel (#|ind_bodies mdecl| - S (inductive_ind ind) + #|ind_params mdecl| + #|arity|) in
+  let s := (inds (inductive_mind ind) u (ind_bodies mdecl)) in
+  inductive_ind ind < #|ind_bodies mdecl| ->
+  subst s (#|arity| + #|ind_params mdecl|)
+        (subst_instance_constr u (mkApps head (to_extended_list_k (ind_params mdecl) #|arity| ++ args)))
+  = mkApps (tInd ind u) (to_extended_list_k (ind_params mdecl) #|arity| ++
+                        map (subst s (#|arity| + #|ind_params mdecl|)) (map (subst_instance_constr u) args)).
+Proof.
+  intros.
+  rewrite subst_instance_constr_mkApps subst_mkApps.
+  f_equal.
+  - subst head. simpl subst_instance_constr.
+    rewrite (subst_rel_eq _ _ (#|ind_bodies mdecl| - S (inductive_ind ind)) (tInd ind u)) //; try lia.
+    subst s. rewrite inds_alt rev_mapi nth_error_mapi /=.
+    elim nth_error_spec. intros. simpl.
+    f_equal. destruct ind; simpl. f_equal. f_equal. simpl in H. lia.
+    rewrite List.rev_length. lia.
+  - rewrite !map_app. f_equal.
+    -- rewrite map_subst_instance_constr_to_extended_list_k.
+       erewrite to_extended_list_k_map_subst at 2.
+       now rewrite Nat.add_comm. lia.
+Qed.
+
+Lemma decompose_app_mkApps f l :
+  isApp f = false -> decompose_app (mkApps f l) = (f, l).
+Proof.
+  intros.
+  destruct l; simpl;
+    destruct f; simpl; try (discriminate || reflexivity).
+Qed.
+
+Fixpoint reln_alt p Γ :=
+  match Γ with
+  | [] => []
+  | {| decl_body := Some _ |} :: Γ => reln_alt (p + 1) Γ
+  | {| decl_body := None |} :: Γ => tRel p :: reln_alt (p + 1) Γ
+  end.
+
+Lemma reln_alt_eq l Γ k : reln l k Γ = List.rev (reln_alt k Γ) ++ l.
+Proof.
+  induction Γ in l, k |- *; simpl; auto.
+  destruct a as [na [body|] ty]; simpl.
+  now rewrite IHΓ.
+  now rewrite IHΓ -app_assoc.
+Qed.
+
+Lemma to_extended_list_k_cons d Γ k :
+  to_extended_list_k (d :: Γ) k =
+  match d.(decl_body) with
+  | None => to_extended_list_k Γ (S k) ++ [tRel k]
+  | Some b => to_extended_list_k Γ (S k)
+  end.
+Proof.
+  rewrite /to_extended_list_k reln_alt_eq. simpl.
+  destruct d as [na [body|] ty]. simpl.
+  now rewrite reln_alt_eq Nat.add_1_r.
+  simpl. rewrite reln_alt_eq.
+  now rewrite -app_assoc !app_nil_r Nat.add_1_r.
+Qed.
+
+Lemma lift_to_extended_list_k Γ k : forall k',
+    to_extended_list_k Γ (k' + k) = map (lift0 k') (to_extended_list_k Γ k).
+Proof.
+  unfold to_extended_list_k.
+  intros k'. rewrite !reln_alt_eq !app_nil_r.
+  induction Γ in k, k' |- *; simpl; auto.
+  destruct a as [na [body|] ty].
+  now rewrite -Nat.add_assoc (IHΓ (k + 1) k').
+  simpl. now rewrite -Nat.add_assoc (IHΓ (k + 1) k') map_app.
+Qed.
+
+Lemma subst_to_extended_list_k s k args ctx :
+  Forall Ast.wf s ->
+  make_context_subst (List.rev ctx) args [] = Some s ->
+  map (subst s k) (to_extended_list_k ctx k) = map (lift0 k) args.
+Proof.
+  move=> wfs.
+  move/make_context_subst_spec. rewrite List.rev_involutive.
+  move=> H; induction H; simpl; auto.
+  - inv wfs.
+    rewrite map_app -IHcontext_subst //.
+    rewrite to_extended_list_k_cons /= !map_app.
+    f_equal.
+    rewrite (lift_to_extended_list_k _ _ 1) map_map_compose.
+    pose proof (to_extended_list_k_spec Γ k).
+    apply_spec. intros x [n [-> Hn]].
+    rewrite /compose /lift (subst_app_decomp [a] s k); auto with wf.
+    rewrite subst_rel_gt. simpl; lia.
+    repeat (f_equal; simpl; try lia).
+    now rewrite /map (subst_rel_eq _ _ 0 a).
+  - inv wfs.
+    rewrite -IHcontext_subst // to_extended_list_k_cons /=.
+    rewrite (lift_to_extended_list_k _ _ 1) map_map_compose.
+    pose proof (to_extended_list_k_spec Γ k).
+    apply_spec. intros x [n [-> Hn]].
+    rewrite /compose /lift (subst_app_decomp [subst0 s b] s k); auto with wf.
+    rewrite subst_rel_gt. simpl; lia.
+    repeat (f_equal; simpl; try lia).
+Qed.
+
+Lemma wf_context_subst ctx args s :
+  Forall wf_decl ctx -> Forall Ast.wf args ->
+  context_subst ctx args s -> Forall Ast.wf s.
+Proof.
+  move=> wfctx wfargs.
+  induction 1. constructor.
+  eapply Forall_app in wfargs as [wfargs wfa]. inv wfa. inv wfctx.
+  constructor; intuition auto.
+  inv wfctx. red in H0. constructor; intuition auto with wf.
+Qed.
+
+Lemma wf_make_context_subst ctx args s' :
+  Forall wf_decl ctx -> Forall Ast.wf args ->
+  make_context_subst (List.rev ctx) args [] = Some s' -> Forall Ast.wf s'.
+Proof.
+  move=> wfctx wfargs.
+  move/make_context_subst_spec. rewrite rev_involutive.
+  eauto using wf_context_subst.
+Qed.
+
+Lemma chop_n_app {A} {l l' : list A} {n} : n = length l -> chop n (l ++ l') = (l, l').
+Proof.
+  intros ->. induction l; simpl; try congruence.
+  now rewrite IHl.
 Qed.
 
 (** check_correct_arity is probably wrong, w.r.t. let-ins reduced or not at least  *)
@@ -1107,15 +1470,14 @@ Lemma subst_types_of_case `{cf:checker_flags} Σ ind mdecl idecl args u p pty in
   wf Σ ->
   Forall Ast.wf n -> Forall Ast.wf args ->
   Ast.wf pty -> Ast.wf (ind_type idecl) ->
-  forall s, context_subst pctx args s ->
-  on_ind_body (lift_typing typing) Σ (inductive_mind ind) mdecl (inductive_ind ind) idecl ->
+  declared_inductive (fst Σ) ind mdecl idecl ->
   types_of_case ind mdecl idecl args u p pty = Some (indctx, pctx, ps, btys) ->
   types_of_case ind mdecl idecl (map (f []) args) u (f [] p) (f [] pty) =
   Some (f_ctx indctx, f_ctx pctx, ps, map (on_snd (f [])) btys).
 Proof.
-  simpl. intros wfΣ wfn wfargs wfpty wfdecl argss wfcsubst wfidecl. simpl.
+  simpl. intros wfΣ wfn wfargs wfpty wfdecl wfidecl. simpl.
   epose proof (subst_declared_inductive _ ind mdecl idecl n k wfΣ).
-  forward H. admit. rewrite <- H at 2.
+  forward H. auto. rewrite <- H at 2.
   unfold types_of_case.
   pose proof (subst_destArity [] (ind_type idecl) n k wfdecl); trivial. simpl in H.
   unfold subst_context, fold_context in H0. simpl in H0. rewrite ind_type_map. simpl.
@@ -1127,6 +1489,12 @@ Proof.
   rewrite H0; clear H0.
   destruct map_option_out eqn:Hbrs; try congruence.
   intros [= -> -> -> ->].
+  pose proof (on_declared_inductive _ _ _ _ wfΣ wfidecl) as [onmind onind].
+  pose proof (onParams _ _ _ _ onmind) as Hparams.
+  assert(closedparams : closed_ctx (ind_params mdecl)).
+  eapply closed_wf_local; eauto.
+  assert(wfparams : Forall wf_decl (ind_params mdecl)).
+  eapply typing_all_wf_decl; eauto.
   assert(forall brs,
          build_branches_type ind mdecl idecl args u p = brs ->
          (build_branches_type ind mdecl
@@ -1137,67 +1505,83 @@ Proof.
   { intros brs <-.
     unfold build_branches_type.
     rewrite ind_ctors_map.
-    rewrite mapi_map, map_mapi.
-    apply onConstructors in wfidecl.
-    red in wfidecl. eapply (Alli_mapi_spec wfidecl). clear wfidecl.
+    rewrite mapi_map map_mapi.
+    apply onConstructors in onind.
+    red in onind. eapply (Alli_mapi_spec onind). clear onind.
     intros i [[id t] arity]. simpl.
     rewrite <- subst_subst_instance_constr.
-    rewrite substl_inds_subst.
+    rewrite -> substl_inds_subst.
     assert (Hn:map (UnivSubst.subst_instance_constr u) n = n). admit.
     rewrite Hn. clear Hn.
     intros Honc.
     pose proof (on_constructor_closed wfΣ (u:=u) Honc).
     simpl in H0.
-    eapply closed_upwards in H0. eapply subst_closedn in H0. rewrite H0.
-    clear H0.
-    destruct Honc as [Ht Hparams]. simpl in *.
-    destruct Hparams. simpl in cshape_eq.
+    rewrite <- subst_instantiate_params; auto with wf.
     remember (substl (inds (inductive_mind ind) u (ind_bodies mdecl)) (subst_instance_constr u t)) as
-        ty. revert Heqty.
-    subst t. unfold substl.
-    rewrite !subst_instance_constr_it_mkProd_or_LetIn, !subst_it_mkProd_or_LetIn.
-    eapply (context_subst_instantiate_params _ _ _ ty) in wfcsubst.
+        ty.
+    destruct (instantiate_params (ind_params mdecl) args ty) eqn:Heq; auto.
+    eapply instantiate_params_make_context_subst in Heq.
+    destruct Heq as [ctx' [ty'' [s' [Hty [Hsubst Ht0]]]]].
+    subst t0. simpl.
 
+    rewrite Heqty in Hty.
+    destruct Honc. destruct c.
+    simpl in *. rewrite cshape_eq in Hty.
+    rewrite -> !subst_instance_constr_it_mkProd_or_LetIn in Hty.
+    unfold substl in Hty. rewrite !subst_it_mkProd_or_LetIn in Hty.
+    assert(#|subst_context (inds (inductive_mind ind) u (ind_bodies mdecl)) 0
+             (subst_instance_context u (ind_params mdecl))| = #|ind_params mdecl|).
+    now rewrite subst_context_length subst_instance_context_length.
+    rewrite <- H1 in Hty.
+    rewrite decompose_prod_n_assum_it_mkProd in Hty.
+    injection Hty. clear Hty.
+    intros Heqty'' <-. revert Heqty''.
+    rewrite !subst_instance_context_length Nat.add_0_r.
 
+    rewrite (subst_cstr_concl_head ind u mdecl cshape_arity cshape_args).
+    destruct wfidecl as [Hmdecl Hnth].
+    now apply nth_error_Some_length in Hnth.
+    intros <-. rewrite !subst_it_mkProd_or_LetIn !subst_mkApps /=.
+    rewrite !decompose_prod_assum_it_mkProd /=; try by rewrite is_ind_app_head_mkApps.
+    rewrite !decompose_app_mkApps; try by reflexivity.
+    simpl. rewrite !map_app !subst_context_length !subst_instance_context_length Nat.add_0_r.
+    rewrite !(subst_to_extended_list_k _ _ args) //.
+    eapply wf_make_context_subst in Hsubst; eauto.
 
-    rewrite !subst_instance_context_length, Nat.add_0_r.
+    pose proof Hsubst as Hsubst'.
+    apply make_context_subst_spec in Hsubst'.
+    rewrite rev_involutive in Hsubst'.
+    pose proof (context_subst_assumptions_length _ _ _ Hsubst').
 
-
-
-
-
-    destruct (instantiate_params _ args) eqn:Heq.
-    rewrite (subst_instantiate_params n k _ _ _ wfn _ Heq).
-    2:{ eapply subst_instantiate_params_none in Heq.
-        rewrite Heq. all:eauto.
-        apply has_nparams_subst. apply has_nparams_subst_instance_constr. admit.
-        apply wf_subst. apply wf_inds. apply wf_subst_instance_constr. red in Ht.
-        red in Ht. destruct Ht as [s'' Hs]. eapply typing_wf in Hs; intuition eauto.
-        apply typing_wf_local in Hs; eauto. }
-
-    destruct (decompose_prod_assum [] t0) eqn:Heq'.
-    destruct (decompose_app t1) as [fn arg] eqn:?.
-
-    rewrite (decompose_app_subst _ _ _ fn arg); auto. simpl. *)
-(*   destruct (chop _ arg) eqn:Heqchop. eapply chop_map in Heqchop. *)
-(*   rewrite Heqchop. clear Heqchop. *)
-(*   unfold on_snd. simpl. f_equal. *)
-(*   rewrite subst_it_mkProd_or_LetIn, !subst_mkApps, map_app; simpl. *)
-(*   rewrite !subst_mkApps, !map_app, subst_context_length. *)
-(*   rewrite permute_subst by lia. repeat f_equal. *)
-(*   now rewrite to_extended_list_subst, <- to_extended_list_map_subst. *)
-(*   simpl. reflexivity. *)
-(*   specialize (H _ eq_refl). rewrite H. clear H. *)
-(*   rewrite map_option_out_map_option_map. *)
-(*   destruct (map_option_out (build_branches_type _ _ _ _ _ _)). *)
-(*   intros [= -> -> -> <-]. reflexivity. congruence. *)
-(* Qed. *)
-(* Admitted. *)
-admit. }
+    symmetry.
+    case E: chop => [l l'].
+    have chopm := (chop_map _ _ _ _ _ E).
+    move: E chopm.
+    rewrite chop_n_app ?map_length.
+    rewrite <- H2. apply onNpars in onmind. lia.
+    move=> [= <- <-] chopm.
+    symmetry.
+    move: {chopm}(chopm _ (subst n (#|cshape_arity| + k))).
+    rewrite map_app.
+    move=> chopm; rewrite {}chopm /=.
+    rewrite !app_nil_r /on_snd /=.
+    rewrite subst_it_mkProd_or_LetIn !subst_context_length !subst_mkApps
+            !subst_instance_context_length !map_app.
+    f_equal. f_equal. f_equal. f_equal.
+    2:{ f_equal. simpl. f_equal.
+        rewrite !subst_mkApps /= !map_app. f_equal.
+        f_equal.
+        rewrite /to_extended_list -to_extended_list_k_map_subst.
+        rewrite !subst_context_length subst_instance_context_length. lia.
+        now rewrite to_extended_list_k_subst. }
+    rewrite commut_lift_subst_rec. lia. reflexivity.
+    unfold substl. apply wf_subst. apply wf_inds. apply wf_subst_instance_constr.
+    destruct Honc as [[s' Hty] _]. simpl in Hty. eapply typing_wf in Hty; intuition eauto with wf.
+    apply Forall_map. eapply Forall_impl; eauto. apply wf_subst_instance_constr. }
   specialize (H0 _ eq_refl). rewrite H0.
   rewrite map_option_out_map_option_map. rewrite Hbrs.
   simpl. f_equal.
-Admitted.
+Admitted. (* only remaining goal is for subst_instance_constr in the substitution n *)
 
 Hint Unfold subst1 : subst.
 Hint Rewrite subst_mkApps distr_subst: subst.
@@ -1254,7 +1638,7 @@ Proof.
   clear -H1.
   unfold is_constructor in *.
   destruct (nth_error l narg) eqn:Heq.
-  eapply nth_error_app_left in Heq. now rewrite Heq. discriminate.
+  eapply nth_error_app_left in Heq. now rewrite -> Heq. discriminate.
 
   intros. rewrite mkApp_mkApps. now constructor.
 
@@ -1314,42 +1698,42 @@ Proof.
     elim (leb_spec_Set); intros Hn.
     + destruct (nth_error s) eqn:Heq.
       ++ pose proof (nth_error_Some_length Heq).
-         rewrite nth_error_app_ge in H by lia.
-         rewrite nth_error_app_lt in H by lia.
+         rewrite -> nth_error_app_ge in H by lia.
+         rewrite -> nth_error_app_lt in H by lia.
          destruct nth_error eqn:HΓ'.
          eapply subs_nth_error in Heq; eauto.
          simpl in H. destruct decl_body; try contradiction.
          discriminate. discriminate.
       ++ apply nth_error_None in Heq.
          assert(S i = #|s| + (S (i - #|s|))) by lia.
-         rewrite H1. rewrite simpl_subst; try lia.
+         rewrite H1. rewrite -> simpl_subst; try lia.
          econstructor.
-         rewrite nth_error_app_ge in H by lia.
-         rewrite nth_error_app_ge in H by lia.
-         rewrite nth_error_app_ge. 2:(autorewrite with wf; lia).
+         rewrite -> nth_error_app_ge in H by lia.
+         rewrite -> nth_error_app_ge in H by lia.
+         rewrite -> nth_error_app_ge. 2:(autorewrite with wf; lia).
          rewrite <- H. f_equal. f_equal. autorewrite with wf. lia.
-         rewrite !nth_error_app_ge in H by lia.
+         rewrite -> !nth_error_app_ge in H by lia.
          destruct nth_error eqn:Hi.
          eapply nth_error_All_local_env in wfΓ. red in wfΓ.
-         rewrite Hi in wfΓ. simpl in H.
+         rewrite -> Hi in wfΓ. simpl in H.
          destruct c; simpl in H; try discriminate.
          injection H. intros ->. red in wfΓ. cbn in *. apply typing_wf in wfΓ. intuition eauto. eauto.
          eapply typing_wf_local in wfΓ; eauto.
          apply nth_error_Some_length in Hi. lia. discriminate.
-    + rewrite nth_error_app_lt in H by lia.
+    + rewrite -> nth_error_app_lt in H by lia.
       pose (commut_lift_subst_rec body s (S i) (#|Γ''| - S i) 0).
       assert(eq:(S i + (#|Γ''| - S i)) = #|Γ''|) by lia.
-      rewrite eq in e. rewrite <- e by lia.
+      rewrite -> eq in e. rewrite <- e by lia.
       constructor.
-      rewrite nth_error_app_lt by (autorewrite with wf; lia).
-      rewrite nth_error_subst_context.
-      unfold subst_decl; now rewrite option_map_decl_body_map_decl, H, Nat.add_0_r.
+      rewrite -> nth_error_app_lt by (autorewrite with wf; lia).
+      rewrite -> nth_error_subst_context.
+      unfold subst_decl; now rewrite -> option_map_decl_body_map_decl, H, Nat.add_0_r.
 
   - rewrite subst_iota_red.
     constructor.
 
   - inv wfM. rewrite mkApps_tApp; simpl; auto with wf.
-    rewrite mkApps_tApp; simpl; auto with wf.
+    rewrite -> mkApps_tApp; simpl; auto with wf.
     eapply red_fix. erewrite subst_unfold_fix; eauto.
     now apply subst_is_constructor.
     inv H3.
@@ -1370,7 +1754,7 @@ Proof.
 
   - inv wfM.
     simpl. constructor.
-    now rewrite nth_error_map, H.
+    now rewrite nth_error_map H.
 
   - constructor.
     inv wfM.
@@ -1429,65 +1813,68 @@ Proof. unfold eq_string. destruct string_dec; congruence. Qed.
 Lemma eq_ind_refl i : eq_ind i i = true.
 Proof.
   destruct i as [mind k].
-  unfold eq_ind. now rewrite eq_string_refl, Nat.eqb_refl.
+  unfold eq_ind. now rewrite eq_string_refl Nat.eqb_refl.
 Qed.
+
+Lemma eq_nat_refl n : eq_nat n n = true.
+Proof. by rewrite /eq_nat Nat.eqb_refl. Qed.
 
 Lemma eq_projection_refl i : eq_projection i i = true.
 Proof.
   destruct i as [[mind k] p].
   unfold eq_projection.
-  now rewrite eq_ind_refl, !Nat.eqb_refl.
+  now rewrite eq_ind_refl !eq_nat_refl.
 Qed.
 
 Lemma eq_term_refl `{checker_flags} φ t : eq_term φ t t = true.
 Proof.
   induction t using term_forall_list_ind; simpl; try reflexivity; try discriminate;
     try (merge_Forall; close_Forall; intuition auto);
-    try (rewrite ?IHt1, ?IHt2, ?IHt3; reflexivity).
+    try (rewrite -> ?IHt1, ?IHt2, ?IHt3; reflexivity).
 
   - apply Nat.eqb_refl.
   - apply eq_string_refl.
   - apply Nat.eqb_refl.
-  - unfold eq_evar. rewrite Nat.eqb_refl.
-    simpl. induction H0; simpl; auto. now rewrite H0, IHForall.
+  - rewrite /eq_evar eq_nat_refl.
+    simpl. induction H0; simpl; auto. now rewrite H0 IHForall.
   - apply eq_universe_refl.
   - rewrite IHt; simpl.
     eapply (Forall_forallb _ _ (fun x => eq_term φ x x)) in H0.
     induction l; simpl; auto.
-    simpl in H0. rewrite andb_true_iff in H0. intuition.
+    simpl in H0. rewrite -> andb_true_iff in H0. intuition.
     auto.
   - unfold eq_constant. rewrite eq_string_refl.
     apply eq_universe_instance_refl.
   - rewrite eq_ind_refl. apply eq_universe_instance_refl.
-  - rewrite eq_ind_refl. rewrite Nat.eqb_refl. apply eq_universe_instance_refl.
+  - rewrite eq_ind_refl. rewrite /eq_nat Nat.eqb_refl. apply eq_universe_instance_refl.
   - destruct p. simpl.
-    rewrite eq_ind_refl, Nat.eqb_refl, IHt1, IHt2.
+    rewrite eq_ind_refl eq_nat_refl IHt1 IHt2.
     simpl. induction l.
     reflexivity.
     simpl. destruct a. inv H0. simpl in H1. rewrite H1.
     rewrite IHl; auto.
-  - now rewrite eq_projection_refl, IHt.
+  - now rewrite eq_projection_refl IHt.
+  - rewrite eq_nat_refl.
+    induction m. reflexivity.
+    inv H0. intuition.
+    simpl. rewrite H0 H3. simpl. apply H1.
   - rewrite Nat.eqb_refl.
     induction m. reflexivity.
     inv H0. intuition.
-    simpl. rewrite H0, H3. simpl. apply H1.
-  - rewrite Nat.eqb_refl.
-    induction m. reflexivity.
-    inv H0. intuition.
-    simpl. rewrite H0, H3. simpl. apply H1.
+    simpl. rewrite H0 H3. simpl. apply H1.
 Qed.
 
 Lemma eq_term_leq_term `{checker_flags} φ t u : eq_term φ t u = true -> leq_term φ t u = true.
 Proof.
   induction t in u |- * using term_forall_list_ind; simpl; intros; auto; try reflexivity; try discriminate;
     try (merge_Forall; close_Forall; intuition auto);
-    try (rewrite ?IHt1, ?IHt2, ?IHt3; reflexivity).
+    try (rewrite -> ?IHt1, ?IHt2, ?IHt3; reflexivity).
 
   - destruct u; auto. now apply eq_universe_leq_universe.
   - destruct u; try discriminate.
-    rewrite andb_true_iff in *. intuition.
+    rewrite -> andb_true_iff in *. intuition.
   - destruct u; try discriminate.
-    rewrite andb_true_iff in *. intuition.
+    rewrite -> andb_true_iff in *. intuition.
 Qed.
 
 Lemma eq_term_App `{checker_flags} φ f f' :
@@ -1506,15 +1893,15 @@ Proof.
   induction l in f, f' |- *; destruct l'; try (simpl; congruence).
   intros.
   destruct (isApp f) eqn:Hf.
-  pose (eq_term_App _ _ _ H0). rewrite Hf in e.
+  pose (eq_term_App _ _ _ H0). rewrite -> Hf in e.
   destruct f; try discriminate.
   destruct f'; try discriminate.
   simpl in *.
-  rewrite andb_true_iff in *. intuition.
+  rewrite -> andb_true_iff in *. intuition.
   rewrite forallb2_app; auto.
-  simpl. now rewrite H3, H0, H4.
+  simpl. now rewrite H3 H0 H4.
 
-  rewrite !mkApps_tApp; auto. simpl. rewrite H0.
+  rewrite -> !mkApps_tApp; auto. simpl. rewrite -> H0.
   apply H1.
   pose proof (eq_term_App _ _ _ H0). all:congruence.
 Qed.
@@ -1528,15 +1915,15 @@ Proof.
   intros. simpl. apply eq_term_leq_term. auto.
   intros.
   destruct (isApp f) eqn:Hf.
-  pose (eq_term_App _ _ _ H0). rewrite Hf in e.
+  pose (eq_term_App _ _ _ H0). rewrite -> Hf in e.
   destruct f; try discriminate.
   destruct f'; try discriminate.
   simpl in *.
-  rewrite andb_true_iff in *. intuition.
+  rewrite -> andb_true_iff in *. intuition.
   rewrite forallb2_app; auto.
-  simpl. now rewrite H3, H0, H4.
+  simpl. now rewrite H3 H0 H4.
 
-  rewrite !mkApps_tApp; auto. simpl. rewrite H0.
+  rewrite -> !mkApps_tApp; auto. simpl. rewrite H0.
   apply H1.
   pose (eq_term_App _ _ _ H0). all:congruence.
 Qed.
@@ -1550,7 +1937,7 @@ Proof.
     destruct U; try discriminate;
   try solve [simpl; auto]; try
                              (destruct (mkApps_trans_wf _ _ H0) as [U' [V' ->]]; reflexivity);
-  simpl in *; revert Hleq; try rewrite !andb_true_iff in *; intuition auto;
+  simpl in *; revert Hleq; try rewrite -> !andb_true_iff in *; intuition auto;
     try (merge_Forall; close_Forall; intuition auto).
 
   - intros.
@@ -1566,12 +1953,12 @@ Proof.
 
   - destruct p. destruct Nat.leb. discriminate. discriminate.
   - destruct p. discriminate.
-  - destruct p, p0. rewrite !andb_true_iff in *. intuition auto.
+  - destruct p, p0. rewrite -> !andb_true_iff in *. intuition auto.
     red in H0. merge_Forall. close_Forall. intuition auto. destruct y. simpl. auto.
-  - rewrite !andb_true_iff in *.
+  - rewrite -> !andb_true_iff in *.
     destruct x, y; simpl in *; intuition auto.
     assert (#|m| = #|m0|). clear -H2. induction H2; simpl; auto. rewrite H4. auto.
-  - rewrite !andb_true_iff in *.
+  - rewrite -> !andb_true_iff in *.
     destruct x, y; simpl in *; intuition auto.
     assert (#|m| = #|m0|). clear -H2. induction H2; simpl; auto. rewrite H4. auto.
 Qed.
@@ -1585,7 +1972,7 @@ Proof.
     destruct U; try discriminate;
   try solve [simpl; auto]; try
                              (destruct (mkApps_trans_wf _ _ H0) as [U' [V' ->]]; reflexivity);
-  simpl in *; revert Hleq; try destruct p, p0; try rewrite !andb_true_iff in *;
+  simpl in *; revert Hleq; try destruct p, p0; try rewrite -> !andb_true_iff in *;
     intuition auto using subst_eq_term;
     try (merge_Forall; close_Forall; intuition eauto using subst_eq_term).
 
@@ -1599,11 +1986,11 @@ Proof.
   - destruct p. discriminate.
   - destruct p; discriminate.
   - destruct y. simpl. auto using subst_eq_term.
-  - rewrite !andb_true_iff in *.
+  - rewrite -> !andb_true_iff in *.
     destruct x, y; simpl in *; intuition auto using subst_eq_term.
     assert (#|m| = #|m0|). clear -H2. induction H2; simpl; auto. rewrite H4.
     auto using subst_eq_term.
-  - rewrite !andb_true_iff in *.
+  - rewrite -> !andb_true_iff in *.
     destruct x, y; simpl in *; intuition auto using subst_eq_term.
     assert (#|m| = #|m0|). clear -H2. induction H2; simpl; auto. rewrite H4.
     auto using subst_eq_term.
@@ -1615,12 +2002,12 @@ Lemma subst_eq_context `{checker_flags} φ l l' n k :
 Proof.
   induction l in l', n, k |- *; intros; destruct l'; rewrite ?subst_context_snoc;
     try (discriminate || reflexivity).
-  simpl in *. rewrite andb_true_iff in *.
+  simpl in *. rewrite -> andb_true_iff in *.
   intuition. unfold eq_context in H2. apply forallb2_length in H2. rewrite <- H2.
   destruct a, c; try congruence.
   unfold eq_decl in *. simpl.
   destruct decl_body, decl_body0; simpl in *; try congruence.
-  simpl in *. rewrite andb_true_iff in *.
+  simpl in *. rewrite -> andb_true_iff in *.
   intuition auto using subst_eq_term.
   intuition auto using subst_eq_term.
 Qed.
@@ -1639,7 +2026,7 @@ Proof.
   destruct pctx in indctx |- *. simpl; try congruence. simpl.
   rewrite subst_context_snoc. simpl.
   unfold eq_context.
-  rewrite !andb_true_iff. intros.
+  rewrite -> !andb_true_iff. intros.
   destruct H. split.
   destruct c. destruct decl_body; try discriminate.
   unfold eq_decl in *. simpl in *.
@@ -1647,12 +2034,13 @@ Proof.
   rewrite <- H1.
   clear H0.
   eapply (subst_eq_term _ s (#|indctx| + k)) in H.
-  rewrite subst_mkApps, map_app in H. simpl in H.
-  rewrite firstn_map. rewrite to_extended_list_subst.
-  erewrite <- (to_extended_list_map_subst s) in H.
+  rewrite subst_mkApps map_app in H. simpl in H.
+  rewrite firstn_map. rewrite /to_extended_list to_extended_list_k_subst.
+  unfold to_extended_list in H.
+  erewrite <- (to_extended_list_k_map_subst s) in H.
   rewrite <- H. f_equal. f_equal. f_equal. rewrite subst_context_length.
-  rewrite !map_map_compose. apply map_ext.
-  intros. unfold compose. now rewrite commut_lift_subst_rec.
+  rewrite -> !map_map_compose. apply map_ext.
+  intros. unfold compose. now rewrite commut_lift_subst_rec. lia.
   eapply subst_eq_context in H0. eapply H0.
 Qed.
 
@@ -1746,8 +2134,8 @@ Proof.
   eapply cumul_trans; eauto.
   econstructor. econstructor. eapply t. eauto. eauto.
   apply IHHU; eauto.
-  rewrite mkApp_tApp; eauto.
-  econstructor; eauto. rewrite Happ; auto. congruence.
+  rewrite -> mkApp_tApp; eauto.
+  econstructor; eauto. congruence.
   econstructor; eauto.
 Qed.
 
@@ -1796,22 +2184,22 @@ Proof.
     elim nth_error_spec.
     + intros x Heq Hlt.
       pose proof (subst_length _ _ _ _ sub).
-      rewrite Typing.nth_error_app_ge in H0 by lia.
-      rewrite Typing.nth_error_app_lt in H0 by lia.
+      rewrite -> Typing.nth_error_app_ge in H0 by lia.
+      rewrite -> Typing.nth_error_app_lt in H0 by lia.
       eapply subs_nth_error in Heq; eauto.
       destruct decl_body; try contradiction.
       cbn -[skipn] in Heq.
       eapply refine_type.
       eapply (weakening _ _ (subst_context s 0 Δ)) in Heq; eauto with wf.
       rewrite subst_context_length in Heq. eapply Heq.
-      unfold substl. rewrite commut_lift_subst_rec by lia.
+      unfold substl. rewrite -> commut_lift_subst_rec by lia.
       rewrite Nat.add_0_r.
       rewrite <- (firstn_skipn (S (n - #|Δ|)) s) at 2.
-      rewrite subst_app_decomp. f_equal.
+      rewrite -> subst_app_decomp. f_equal.
       replace (S n) with ((S n - #|Δ|) + #|Δ|) by lia.
       assert (eq:#|(map (lift0 #|skipn (S (n - #|Δ|)) s|) (firstn (S (n - #|Δ|)) s))| = S n - #|Δ|).
-      rewrite map_length. rewrite firstn_length by lia. lia.
-      rewrite <- eq. rewrite simpl_subst_rec; auto; try lia.
+      rewrite map_length. rewrite -> firstn_length by lia. lia.
+      rewrite <- eq. rewrite -> simpl_subst_rec; auto; try lia.
       auto with wf. eapply subs_wf in sub; eauto.
       now apply Forall_firstn.
 
@@ -1821,8 +2209,8 @@ Proof.
       assert (S n = #|s| + (S (n - #|s|))) by lia.
       rewrite H2. rewrite simpl_subst; auto; try lia.
       constructor; auto.
-      rewrite nth_error_app_ge; rewrite subst_context_length.
-      rewrite 2!nth_error_app_ge in H0 by lia.
+      rewrite -> nth_error_app_ge; try lia; rewrite subst_context_length.
+      rewrite -> 2!nth_error_app_ge in H0 by lia.
       rewrite <- H0. f_equal. lia.
       lia.
 
@@ -1830,7 +2218,7 @@ Proof.
       rewrite H0 in sub. simpl in sub.
       eapply refine_type. constructor; eauto.
       rewrite <- map_decl_type.
-      rewrite commut_lift_subst_rec by lia.
+      rewrite -> commut_lift_subst_rec by lia.
       f_equal. lia.
 
   - econstructor; auto. eapply X0; eauto.
@@ -1866,7 +2254,7 @@ Proof.
       with (subst s0 #|Δ| (tProd na A B)).
     eapply substitution_cumul; eauto.
     eapply typing_wf in typrod; eauto. intuition.
-    unfold subst1 in IHX1 |- *. rewrite distr_subst in IHX1.
+    unfold subst1 in IHX1 |- *. rewrite -> distr_subst in IHX1.
     apply IHX1.
     apply wf_subst. constructor; auto.
     now apply typing_wf in ty.
@@ -1881,9 +2269,9 @@ Proof.
     assert (s = map (UnivSubst.subst_instance_constr u) s). admit.
     rewrite H1.
     rewrite UnivSubst.subst_subst_instance_constr. f_equal.
-    eapply subst_declared_inductive in isdecl.
-    erewrite <- (ind_type_map (fun Γ t => subst s (#|Γ| + #|Δ|) t)).
-    f_equal. symmetry. apply isdecl. eauto.
+    eapply subst_declared_inductive in isdecl; eauto.
+    erewrite <- (ind_type_map (fun Γ t => subst s (Γ + #|Δ|) t)).
+    f_equal. symmetry. apply isdecl.
 
   - eapply refine_type. econstructor; eauto.
     assert (s = map (UnivSubst.subst_instance_constr u) s). admit.
@@ -1892,26 +2280,21 @@ Proof.
     (* eauto with wf. loops!*)
     eauto using subs_wf.
 
-  - rewrite subst_mkApps, map_app, map_skipn.
+  - rewrite subst_mkApps map_app map_skipn.
     specialize (X1 Γ Γ' Δ s sub eq_refl wfsubs).
     specialize (X4 Γ Γ' Δ s sub eq_refl wfsubs).
     specialize (X2 Γ Γ' Δ s sub eq_refl wfsubs).
     simpl. econstructor.
     5:{ eapply subst_types_of_case in H3.
         simpl in H3. subst pars. rewrite firstn_map. eapply H3; eauto.
-        -- now apply subs_wf in sub.
+        all:eauto.
         -- now apply subs_wf in sub.
         -- subst pars. eapply Forall_firstn.
            apply typing_wf in X3 as [_ X3]; eauto.
            now apply wf_mkApps_inv in X3.
         -- eapply typing_wf in X0; wf.
-        -- eapply typing_wf_sigma in wfΣ.
-           red in H0.
-           eapply (lookup_on_global_env _ _ _ _ wfΣ) in H0 as [Σ' [wfΣ' H0]]; eauto.
-           destruct H1.
-           eapply (nth_error_alli H6) in H0. apply onArity in H0; red in H0. wf.
-        -- apply declared_inductive_inv; eauto.
-           apply weaken_env_prop_typing. }
+        -- eapply on_declared_inductive in H1 as [Hmdecl Hidecl]; auto.
+           apply onArity in Hidecl as [[s' Hty] _]. now eapply typing_wf in Hty; eauto. }
     -- eauto.
     -- eauto.
     -- eauto.
@@ -1936,7 +2319,7 @@ Proof.
     rewrite map_rev. subst ty.
     assert (eqs: s = map (UnivSubst.subst_instance_constr u) s). admit.
     rewrite eqs.
-    rewrite List.rev_length, UnivSubst.subst_subst_instance_constr.
+    rewrite List.rev_length UnivSubst.subst_subst_instance_constr.
     rewrite <- eqs.
     unfold substl. f_equal. f_equal.
     eapply subst_declared_projection in isdecl. 2:eauto.
@@ -1951,16 +2334,16 @@ Proof.
     induction 1; simpl; auto.
     + destruct t0 as [Ht IHt].
       specialize (IHt Γ Γ' (Δ ,,, Γ0) s sub). forward IHt. now rewrite app_context_assoc.
-      rewrite app_context_length, subst_context_app, app_context_assoc, Nat.add_0_r in IHt.
+      rewrite app_context_length subst_context_app app_context_assoc Nat.add_0_r in IHt.
       unfold snoc; rewrite subst_context_snoc; econstructor; auto;
         apply IHt; apply All_local_env_app_inv; intuition.
     + destruct t0 as [Ht IHt].
        specialize (IHt Γ Γ' (Δ ,,, Γ0) s sub). forward IHt. now rewrite app_context_assoc.
-       rewrite app_context_length, subst_context_app, app_context_assoc, Nat.add_0_r in IHt.
+       rewrite app_context_length subst_context_app app_context_assoc Nat.add_0_r in IHt.
        unfold snoc; rewrite subst_context_snoc; econstructor; auto;
        apply IHt; apply All_local_env_app_inv; intuition.
     + erewrite map_dtype. eapply type_Fix.
-      * rewrite nth_error_map, H0. reflexivity.
+      * rewrite nth_error_map H0. reflexivity.
       * now rewrite subst_fix_context.
       * rewrite subst_fix_context.
         apply All_map.
@@ -1971,9 +2354,9 @@ Proof.
         forward IH by now rewrite app_context_assoc.
         rewrite subst_context_app in IH.
         subst types.
-        rewrite !app_context_assoc, Nat.add_0_r, !app_context_length, fix_context_length in IH.
+        rewrite !app_context_assoc Nat.add_0_r !app_context_length fix_context_length in IH.
         specialize (IH X1).
-        rewrite subst_context_length, fix_context_length.
+        rewrite subst_context_length fix_context_length.
         now rewrite commut_lift_subst_rec.
         now apply isLambda_subst.
 
@@ -1986,16 +2369,16 @@ Proof.
     induction 1; simpl; auto.
     + destruct t0 as [Ht IHt].
       specialize (IHt Γ Γ' (Δ ,,, Γ0) s sub). forward IHt. now rewrite app_context_assoc.
-      rewrite app_context_length, subst_context_app, app_context_assoc, Nat.add_0_r in IHt.
+      rewrite app_context_length subst_context_app app_context_assoc Nat.add_0_r in IHt.
       unfold snoc; rewrite subst_context_snoc; econstructor; auto;
         apply IHt; apply All_local_env_app_inv; intuition.
     + destruct t0 as [Ht IHt].
        specialize (IHt Γ Γ' (Δ ,,, Γ0) s sub). forward IHt. now rewrite app_context_assoc.
-       rewrite app_context_length, subst_context_app, app_context_assoc, Nat.add_0_r in IHt.
+       rewrite app_context_length subst_context_app app_context_assoc Nat.add_0_r in IHt.
        unfold snoc; rewrite subst_context_snoc; econstructor; auto;
        apply IHt; apply All_local_env_app_inv; intuition.
     + erewrite map_dtype. eapply type_CoFix.
-      * rewrite nth_error_map, H0. reflexivity.
+      * rewrite nth_error_map H0. reflexivity.
       * now rewrite subst_fix_context.
       * rewrite subst_fix_context.
         apply All_map.
@@ -2006,9 +2389,9 @@ Proof.
         forward IH by now rewrite app_context_assoc.
         rewrite subst_context_app in IH.
         subst types.
-        rewrite !app_context_assoc, Nat.add_0_r, !app_context_length, fix_context_length in IH.
+        rewrite !app_context_assoc Nat.add_0_r !app_context_length fix_context_length in IH.
         specialize (IH X1).
-        rewrite subst_context_length, fix_context_length.
+        rewrite subst_context_length fix_context_length.
         now rewrite commut_lift_subst_rec.
 
   - econstructor; eauto.
